rt spec+proof: add sorted_ipc_queues invariant
This adds the invariant sorted_ipc_queues, which states that the ipc
queues are sorted by the priority of the TCB. More specifically,
the queues are nonincreasing with respect to the priority of the TCB.

This additionally uses the filter operation in the specification
of tcb_ep_append and tcb_ep_dequeue.

Signed-off-by: Michael McInerney <michael.mcinerney@proofcraft.systems>

spec/haskell/src/SEL4/Object/Notification.lhs
@@ -33,6 +33,7 @@ This module specifies the behavior of notification objects.
 > import Data.Bits
 > import Data.List
 > import Data.Maybe(fromJust)
+> import Data.Helpers (mapMaybe, distinct)
 
 \end{impdetails}
 
@@ -135,6 +136,7 @@ If the notification object is already waiting, the current thread is blocked and
 
 >             WaitingNtfn queue -> case isBlocking of
 >                 True -> do
+>                       assert (distinct queue) "queue must be a list of distinct pointers"
 >                       setThreadState (BlockedOnNotification {
 >                                          waitingOnNotification = ntfnPtr } ) thread
 >                       qs' <- tcbEPAppend thread queue
@@ -165,6 +167,7 @@ If a notification object is deleted, then pending receive operations must be can
 >         ntfn <- getNotification ntfnPtr
 >         case ntfnObj ntfn of
 >             WaitingNtfn queue -> do
+>                 assert (distinct queue) "queue must be a list of distinct pointers"
 >                 setNotification ntfnPtr (ntfn { ntfnObj = IdleNtfn })
 >                 forM_ queue (\t -> do
 >                     setThreadState Restart t
@@ -185,6 +188,7 @@ The following function will remove the given thread from the queue of the notifi
 >         ntfn <- getNotification ntfnPtr
 >         assert (isWaiting (ntfnObj ntfn))
 >             "cancelSignal: notification object must be waiting"
+>         assert (distinct (ntfnQueue (ntfnObj ntfn))) "the notification queue must be a list of distinct pointers"
 >         let queue' = delete threadPtr $ ntfnQueue $ ntfnObj ntfn
 >         ntfn' <- case queue' of
 >             [] -> return $ IdleNtfn
